src/Init/Data/Sigma.lean
@@ -1,0 +1,26 @@
+/-
+Copyright (c) 2025 Robin Arnez. All rights reserved.
+Released under Apache 2.0 license as described in the file LICENSE.
+Author: Robin Arnez
+-/
+module
+
+prelude
+public import Init.SimpLemmas
+public import Init.NotationExtra
+
+public section
+
+namespace Sigma
+
+variable {α : Type u} {β : α → Type v}
+
+@[simp]
+protected theorem «forall» {p : (a : α) × β a → Prop} : (∀ x, p x) ↔ ∀ a b, p ⟨a, b⟩ :=
+  ⟨fun h a b => h ⟨a, b⟩, fun h ⟨a, b⟩ => h a b⟩
+
+@[simp]
+protected theorem «exists» {p : (a : α) × β a → Prop} : (∃ x, p x) ↔ ∃ a b, p ⟨a, b⟩ :=
+  ⟨fun ⟨⟨a, b⟩, h⟩ => ⟨a, b, h⟩, fun ⟨a, b, h⟩ => ⟨⟨a, b⟩, h⟩⟩
+
+end Sigma
